Make more generated function always revealed

Source/DafnyCore/Verifier/BoogieGenerator.Functions.cs
@@ -813,6 +813,7 @@ public partial class BoogieGenerator {
         RequiresName(f), new List<Bpl.TypeVariable>(),
         funcFormals.ConvertAll(v => (Bpl.Variable)BplFormalVar(null, v.TypedIdent.Type, true)),
         BplFormalVar(null, Bpl.Type.Bool, false));
+      precondF.AlwaysRevealed = true;
       sink.AddTopLevelDeclaration(precondF);
 
       var appl = FunctionCall(f.tok, RequiresName(f), Bpl.Type.Bool, reqFuncArguments);
